ConcreteSemantics/Basic.lean
@@ -6,13 +6,11 @@ import ConcreteSemantics.BigStep
 
 /-- skip に関する inversion rule -/
 @[simp] theorem BigStep.skip_iff {s t : State} : (Stmt.skip, s) ==> t ↔ t = s := by
-  constructor
-  · intro h
-    cases h
+  constructor <;> intro h
+  · cases h
     rfl
-  · intro h
-    rw [h]
-    apply BigStep.skip
+  · rw [h]
+    big_step
 
 /-- seq に関する inversion rule -/
 @[simp] theorem BigStep.seq_iff {S T s u} :
@@ -26,4 +24,26 @@ import ConcreteSemantics.BigStep
 
   case mpr =>
     obtain ⟨t, hS, hT⟩ := h
-    exact BigStep.seq _ _ _ _ u hS hT
+    big_step
+
+/-- if に関する inversion rule -/
+@[simp] theorem BigStep.if_iff {B S T s t} : (ifThenElse B S T, s) ==> t ↔
+    (B s ∧ (S, s) ==> t) ∨ (¬ B s ∧ (T, s) ==> t) := by
+  constructor <;> intro h
+  · cases h <;> simp_all
+  · rcases h with ⟨hcond, hbody⟩ | ⟨hcond, hbody⟩
+    · big_step
+    · big_step
+
+/-- while に関する inversion rule -/
+theorem BigStep.while_iff {B S s u} : (whileDo B S, s) ==> u ↔
+    (∃ t, B s ∧ (S, s) ==> t ∧ (whileDo B S, t) ==> u) ∨ (¬ B s ∧ u = s) := by
+  constructor <;> intro h
+  · by_cases hcond : B s
+    case pos =>
+      left
+      simp_all only [true_and]
+      sorry
+    case neg =>
+      sorry
+  sorry
